selection sort changes

src/SelectionSort.lean
@@ -1,7 +1,9 @@
 
 import Mathlib.Tactic.Lemma    --For lemma keyword
-import Mathlib.Tactic.Basic    --For simp, linarith, etc.
-
+import Mathlib.Tactic.Basic
+import Mathlib.Tactic.Linarith  --Forces simp to use linarith
+import Mathlib.Logic.Basic
+import Mathlib.Data.List.MinMax
 
 theorem mem_implies_erase_smaller (l : List Nat) (x : Nat) :
 x ∈ l -> sizeOf (l.erase x) < sizeOf l := by
@@ -12,5 +14,57 @@ x ∈ l -> sizeOf (l.erase x) < sizeOf l := by
   . case cons h t ih =>
     simp at h
     cases h
-    . case inl h =>
-      simp [<-h, List.erase]
+    . case inl H =>
+      simp [<-H, List.erase]
+    . case inr H =>
+      simp [ih H]
+      simp [List.erase, H]
+      by_cases H2 : (h == x)
+      . case pos =>
+        simp [H2]
+      . case neg =>
+        simp [H2]
+        simp [Nat.add_lt_add_iff_left, ih H]
+
+def selection_sort (l : List Nat) : List Nat :=
+match H : l.minimum with
+| none => []
+| some m =>
+  m :: selection_sort (l.erase m)
+decreasing_by
+  all_goals simp_wf
+  apply mem_implies_erase_smaller
+  apply List.minimum_mem
+  exact H
+
+#eval selection_sort [3, 2, 1, 4, 5, 6, 7, 8, 9, 10]
+
+--Predicate for a list being sorted
+def sorted : List Nat -> Prop
+--An empty list is sorted
+| [] => True
+--A list containing a single element is sorted
+| [_] => True
+--A list with more than 2 elements is only sorted if all
+--elements are ordered.
+| h1 :: h2 :: t => h1 ≤ h2 ∧ sorted (h2 :: t)
+
+theorem sort_sorted (l : List Nat) :
+sorted (selection_sort l) := by
+  induction l
+  . case nil =>
+    simp [selection_sort, sorted]
+  . case cons h t ih =>
+    cases H : (h::t).minimum
+    . case none =>
+      rw [selection_sort, H]
+      simp [sorted]
+    . case some m =>
+      rw [selection_sort, H]
+      simp
+      by_cases H2: List.minimum (h::t) = h
+      . case pos =>
+        have T : m = h := sorry --follows from H2
+        simp [T, List.erase]
+        sorry
+      . case neg =>
